1. $ f(x) = 2\sqrt{x + 1} + 3 $
2. $ f(x) = 3\sqrt{2x - 5} - 4 $
3. $ f(x) = -4\sqrt{-x + 6} + 2 $
4. $ f(x) = 5\sqrt{3x + 7} $
5. $ f(x) = -2\sqrt{4x - 1} + 3 $
6. $ f(x) = 6\sqrt{-2x + 5} $
7. $ f(x) = 2\sqrt{5x + 3} - 1 $
8. $ f(x) = -3\sqrt{-x + 4} + 6 $
9. $ f(x) = 7\sqrt{3x - 2} $
10. $ f(x) = -4\sqrt{5x + 6} + 3 $
11. $ f(x) = 8\sqrt{2x - 7} - 2 $
12. $ f(x) = -5\sqrt{4x + 1} $
13. $ f(x) = 9\sqrt{-3x + 5} + 4 $
14. $ f(x) = -6\sqrt{2x + 6} $
15. $ f(x) = 3\sqrt{7x - 4} - 5 $
16. $ f(x) = -7\sqrt{5x + 8} + 2 $
17. $ f(x) = 4\sqrt{-x + 3} $
18. $ f(x) = -8\sqrt{2x - 6} + 1 $
19. $ f(x) = 5\sqrt{4x + 7} - 3 $
20. $ f(x) = -9\sqrt{3x - 5} $
21. $ f(x) = 10\sqrt{x + 9} + 2 $
22. $ f(x) = -6\sqrt{4x + 2} - 4 $
23. $ f(x) = 11\sqrt{5x - 3} $
24. $ f(x) = -7\sqrt{3x + 4} + 3 $
25. $ f(x) = 12\sqrt{-2x + 8} - 1 $
26. $ f(x) = 2\sqrt{6x + 5} $
27. $ f(x) = -8\sqrt{5x - 2} + 4 $
28. $ f(x) = 13\sqrt{4x + 7} - 6 $
29. $ f(x) = -9\sqrt{-x + 5} $
30. $ f(x) = 14\sqrt{3x + 6} + 2 $
31. $ f(x) = -10\sqrt{7x - 3} $
32. $ f(x) = 15\sqrt{2x + 4} - 5 $
33. $ f(x) = -11\sqrt{6x + 9} + 1 $
34. $ f(x) = 3\sqrt{-5x + 2} $
35. $ f(x) = -12\sqrt{3x + 5} + 3 $
36. $ f(x) = 16\sqrt{4x - 7} - 4 $
37. $ f(x) = -13\sqrt{5x + 6} $
38. $ f(x) = 17\sqrt{2x + 8} + 3 $
39. $ f(x) = -14\sqrt{-x + 5} - 1 $
40. $ f(x) = 18\sqrt{3x + 2} $
41. $ f(x) = -15\sqrt{4x - 6} + 5 $
42. $ f(x) = 2\sqrt{5x + 3} - 4 $
43. $ f(x) = -16\sqrt{-3x + 7} + 2 $
44. $ f(x) = 19\sqrt{6x - 5} $
45. $ f(x) = -17\sqrt{4x + 9} - 3 $
46. $ f(x) = 20\sqrt{x + 7} $
47. $ f(x) = -18\sqrt{2x + 4} + 1 $
48. $ f(x) = 5\sqrt{3x - 2} - 5 $
49. $ f(x) = -19\sqrt{4x + 6} $
50. $ f(x) = 21\sqrt{-5x + 3} + 4 $
51. $ f(x) = -6\sqrt{2x + 8} - 2 $
52. $ f(x) = 22\sqrt{3x - 4} $
53. $ f(x) = -20\sqrt{5x + 9} + 1 $
54. $ f(x) = 23\sqrt{-4x + 2} - 3 $
55. $ f(x) = -21\sqrt{6x + 7} + 5 $
56. $ f(x) = 24\sqrt{2x - 8} $
57. $ f(x) = -22\sqrt{3x + 5} - 4 $
58. $ f(x) = 25\sqrt{4x - 1} + 2 $
59. $ f(x) = -23\sqrt{-5x + 6} $
60. $ f(x) = 26\sqrt{7x + 3} - 6 $
61. $ f(x) = -24\sqrt{6x - 2} $
62. $ f(x) = 3\sqrt{-x + 9} + 4 $
63. $ f(x) = -25\sqrt{4x + 8} $
64. $ f(x) = 27\sqrt{3x - 7} - 1 $
65. $ f(x) = -26\sqrt{2x + 4} + 2 $
66. $ f(x) = 28\sqrt{5x + 1} $
67. $ f(x) = -27\sqrt{-4x + 6} - 3 $
68. $ f(x) = 29\sqrt{3x + 2} + 5 $
69. $ f(x) = -28\sqrt{7x - 3} $
70. $ f(x) = 30\sqrt{2x + 7} - 4 $
71. $ f(x) = -29\sqrt{6x + 5} $
72. $ f(x) = 4\sqrt{5x - 8} + 3 $
73. $ f(x) = -30\sqrt{3x + 6} $
74. $ f(x) = 31\sqrt{-x + 2} - 2 $
75. $ f(x) = -32\sqrt{4x + 9} $
76. $ f(x) = 6\sqrt{3x - 7} + 1 $
77. $ f(x) = -33\sqrt{2x + 8} $
78. $ f(x) = 34\sqrt{-5x + 4} - 5 $
79. $ f(x) = -35\sqrt{4x + 1} $
80. $ f(x) = 8\sqrt{3x + 7} + 2 $
81. $ f(x) = -36\sqrt{5x - 3} $
82. $ f(x) = 37\sqrt{2x + 5} - 6 $
83. $ f(x) = -38\sqrt{6x + 2} + 4 $
84. $ f(x) = 9\sqrt{-x + 9} $
85. $ f(x) = -39\sqrt{3x + 5} + 3 $
86. $ f(x) = 40\sqrt{4x - 2} - 1 $
87. $ f(x) = -41\sqrt{2x + 7} + 5 $
88. $ f(x) = 42\sqrt{-3x + 4} $
89. $ f(x) = -43\sqrt{5x + 8} - 3 $
90. $ f(x) = 44\sqrt{2x - 5} + 2 $
91. $ f(x) = -45\sqrt{4x + 3} - 4 $
92. $ f(x) = 46\sqrt{-x + 6} + 1 $